add proof about image.

img_example.v
@@ -8,11 +8,18 @@ Import Prenex Implicits.
 
 Require Import Coq.Sets.Image.
 
+(* R2 島内剛一 数学の基礎 *)
+(* R3 斎藤正彦 数学の基礎 ISBN 4-13-062909-3 *)
+
 Section ImgExample.
   Variable U V:Type.
 
   Import SetNotations.
 
+  (* R3 1.2.4 definition *)
+  Inductive InvIm (B: Ensemble V) (f:U -> V): Ensemble U :=
+    InvIm_intro: forall (x:U), (f x) ∈ B -> x ∈ (InvIm B f).
+  
   Notation "ℑ𝔪( f | A )" := (Im _ _ A f) (at level 60).
 
   Lemma Img_Subset: forall (A B:Ensemble U) (f: U -> V),
@@ -50,5 +57,21 @@ Section ImgExample.
     right.
     apply H.
   Qed.
-  
+
+  (* R2 Problem 2.3.9 *)
+  Lemma Img_Intersection: forall (A B:Ensemble U) (f: U -> V),
+      ℑ𝔪( f | A ∩ B ) ⊂ ℑ𝔪( f | A ) ∩ ℑ𝔪( f | B ).
+  Proof.
+    move => A B f x.
+    case => s.
+    case => t HA HB y H0.
+    rewrite H0.
+    split; apply Im_def.
+    apply HA.
+    apply HB.
+  Qed.
+
+  Check InvIm.
+  Goal forall (A:Ensemble U) (f:U->V), A ⊂ InvIm (ℑ𝔪( f | A )) f. 
+
 End ImgExample.
